intermediate/Veritas.Intermediate.Verify.fsti
@@ -306,6 +306,8 @@ let vevictm #vcfg (s:slot_id vcfg) (s':slot_id vcfg) (vs: vtls vcfg {Valid? vs})
           if k2 <> k then Failed
           (* if s' does not point to s in direction d then Fail *)
           else if points_to_some_slot st s' d && pointed_slot st s' d <> s then Failed
+          (* if s has a parent that is different from s' then Fail *)
+          else if has_parent st s && (parent_slot st s <> s' || parent_dir st s <> d) then Failed
           else
             let v'_upd = Spec.update_merkle_value v' d k h false in
             let st_upd = update_value st s' (MVal v'_upd) in
@@ -393,6 +395,7 @@ let vevictbm #vcfg (s:slot_id vcfg) (s':slot_id vcfg) (t:timestamp) (vs:vtls vcf
           if k2 <> k || b2 then Failed
           (* if s' does not point to s in direction d then Fail *)
           else if not (points_to_dir st s' d s) then Failed
+          else if not (has_parent st s) || parent_slot st s <> s' || parent_dir st s <> d then Failed
           else
             (* update the evict hash and the clock *)
             let vs = vevictb_update_hash_clock s t vs in
